<?xml version="1.0"?>
<rdf:RDF xmlns="http://www.ease-crc.org/ont/SOMA-NEEM.owl#"
     xml:base="http://www.ease-crc.org/ont/SOMA-NEEM.owl"
     xmlns:dc="http://purl.org/dc/elements/1.1/"
     xmlns:owl="http://www.w3.org/2002/07/owl#"
     xmlns:rdf="http://www.w3.org/1999/02/22-rdf-syntax-ns#"
     xmlns:xml="http://www.w3.org/XML/1998/namespace"
     xmlns:xsd="http://www.w3.org/2001/XMLSchema#"
     xmlns:SOMA="http://www.ease-crc.org/ont/SOMA.owl#"
     xmlns:rdfs="http://www.w3.org/2000/01/rdf-schema#">
    <owl:Ontology rdf:about="http://www.ease-crc.org/ont/SOMA-NEEM.owl">
        <owl:imports rdf:resource="http://www.ease-crc.org/ont/SOMA.owl"/>
        <rdfs:comment>SOMA-NEEM.owl defines concepts useful to describe metadata associated to a NEEM, such as the recorded media that it includes.</rdfs:comment>
    </owl:Ontology>
    


    <!-- 
    ///////////////////////////////////////////////////////////////////////////////////////
    //
    // Classes
    //
    ///////////////////////////////////////////////////////////////////////////////////////
     -->

    


    <!-- http://www.ease-crc.org/ont/SOMA.owl#KinoDynamicData -->

    <owl:Class rdf:about="http://www.ease-crc.org/ont/SOMA.owl#KinoDynamicData">
        <rdfs:subClassOf rdf:resource="http://www.ontologydesignpatterns.org/ont/dul/DUL.owl#InformationObject"/>
        <rdfs:subClassOf>
            <owl:Restriction>
                <owl:onProperty rdf:resource="http://www.ontologydesignpatterns.org/ont/dul/DUL.owl#isAbout"/>
                <owl:allValuesFrom rdf:resource="http://www.ontologydesignpatterns.org/ont/dul/DUL.owl#PhysicalObject"/>
            </owl:Restriction>
        </rdfs:subClassOf>
        <rdfs:comment>An InformationObject containing data about how a physical object is put together such that its parts may move relative to each other, and what the physical characteristics of those parts are.</rdfs:comment>
        <rdfs:label xml:lang="en">Kino-dynamic data</rdfs:label>
    </owl:Class>
    


    <!-- http://www.ease-crc.org/ont/SOMA.owl#MeshShapeData -->

    <owl:Class rdf:about="http://www.ease-crc.org/ont/SOMA.owl#MeshShapeData">
        <rdfs:subClassOf rdf:resource="http://www.ontologydesignpatterns.org/ont/dul/DUL.owl#InformationObject"/>
        <rdfs:subClassOf>
            <owl:Restriction>
                <owl:onProperty rdf:resource="http://www.ontologydesignpatterns.org/ont/dul/DUL.owl#isAbout"/>
                <owl:allValuesFrom rdf:resource="http://www.ontologydesignpatterns.org/ont/dul/DUL.owl#PhysicalObject"/>
            </owl:Restriction>
        </rdfs:subClassOf>
        <rdfs:comment>An InformationObject containing data about the geometry of a physical object.</rdfs:comment>
        <rdfs:label xml:lang="en">Mesh-shape data</rdfs:label>
    </owl:Class>
    


    <!-- http://www.ease-crc.org/ont/SOMA.owl#VideoData -->

    <owl:Class rdf:about="http://www.ease-crc.org/ont/SOMA.owl#VideoData">
        <rdfs:subClassOf rdf:resource="http://www.ontologydesignpatterns.org/ont/dul/DUL.owl#InformationObject"/>
        <rdfs:comment>An information object containing data for audio-visual modalities.</rdfs:comment>
        <rdfs:label xml:lang="en">Video data</rdfs:label>
    </owl:Class>
</rdf:RDF>



<!-- Generated by the OWL API (version 4.5.9.2019-02-01T07:24:44Z) https://github.com/owlcs/owlapi -->

